theories/interop/basics_resources.v
@@ -75,6 +75,58 @@ Proof using.
   apply lloc_map_pubs_lookup_None; eauto.
 Qed.
 
+Lemma lloc_own_allocate γGS χ γ:
+  ⌜χ !! γ = None⌝     -∗
+  lloc_own_auth γGS χ ==∗
+  lloc_own_auth γGS (<[γ:=LlocPrivate]> χ) ∗ lloc_own_priv γGS γ.
+Proof using.
+  iIntros (Hne) "Hχ".
+  iNamed "Hχ".
+  iMod (ghost_map_insert with "Hχgmap") as "[Hχmap Hγ]"; first done.
+  iModIntro. iSplitR "Hγ"; last done.
+  iSplitL "Hχmap"; first done. unfold named.
+  rewrite lloc_map_pubs_insert_priv delete_notin.
+  2: destruct (lloc_map_pubs χ !! γ) eqn:Heq; try done; apply lloc_map_pubs_lookup_Some in Heq; congruence.
+  done.
+Qed.
+
+Lemma lloc_own_insert γGS χ γ v:
+  ⌜χ !! γ = None⌝     -∗
+  lloc_own_auth γGS χ ==∗
+  lloc_own_auth γGS (<[γ:=v]> χ).
+Proof using.
+  iIntros (Hne) "Hχ".
+  iMod (lloc_own_allocate with "[] Hχ") as "(Hχ & Hγp)"; first done.
+  destruct v as [l|]; last by iModIntro.
+  iMod (lloc_own_expose with "Hχ Hγp") as "(H & _)". rewrite insert_insert; done.
+Qed.
+
+Lemma lloc_own_mono γGS χ1 χ2 : 
+  lloc_map_mono χ1 χ2  →
+  lloc_own_auth γGS χ1 ==∗
+  lloc_own_auth γGS χ2.
+Proof.
+  intros (Hmono & Hinj).
+  pose (χ2 ∖ χ1) as χdiff.
+  assert (χ1 ##ₘ χdiff) as Hdis by by apply map_disjoint_difference_r.
+  assert (χ2 = (χ1 ∪ χdiff)) as Heq by by rewrite map_difference_union.
+  rewrite Heq in Hinj. rewrite Heq. clear Heq Hmono.
+  revert Hinj Hdis.
+  induction χdiff as [|k v χdiff Hne IH] using map_ind; intros Hinj Hdisj.
+  1: rewrite map_union_empty; iIntros "$ !>"; done.
+  iIntros "Hown".
+  assert (χ1 !! k = None ∧ χ1 ##ₘ χdiff) as [Hnone Hdisj2] by by apply map_disjoint_insert_r in Hdisj.
+  rewrite <- insert_union_r in Hinj; last done.
+  iMod (IH with "[Hown]") as "Hown".
+  1: intros i v1 v2 H1 H2; eapply Hinj; (erewrite lookup_insert_ne; first done); intros <-.
+  1-2: apply elem_of_dom_2 in H1,H2; eapply not_elem_of_dom in Hne,Hnone; rewrite dom_union_L in H1,H2; set_solver.
+  1: done.
+  1: done.
+  rewrite <- insert_union_r; last done.
+  iMod (lloc_own_insert with "[] Hown") as "$"; last done.
+  iPureIntro; apply lookup_union_None; done.
+Qed.
+
 (* Ghost state for [lstore] *)
 
 Definition lstore_own_elem (γGS : gname) (γ : lloc) (dq : dfrac) (b : block) :=
@@ -185,6 +237,26 @@ Proof using.
     rewrite /lstore_own_elem Hmut. iFrame "Helt".
     iModIntro. rewrite lstore_immut_blocks_insert_immut // big_sepM_insert; eauto.
     iFrame. rewrite /lstore_own_immut /lstore_own_elem Hmut //. eauto. }
+Qed.
+
+Lemma lstore_own_insert_many γGS ζ ζnew :
+  ζ ##ₘ ζnew →
+  lstore_own_auth γGS ζ ==∗
+  lstore_own_auth γGS (ζ ∪ ζnew) ∗ [∗ map] γ ↦ b ∈ ζnew, lstore_own_elem γGS γ (DfracOwn 1) b.
+Proof using.
+  induction ζnew as [|γ b ζnew Hne IH] using map_ind.
+  1: intros _; rewrite map_union_empty; iIntros "H !>"; iPoseProof (bi.emp_sep_1 with "H") as "(Hemp&H)"; iFrame "H"; iApply big_sepM_empty; done.
+  iIntros (Hdisj) "Hown".
+  iMod (IH with "Hown") as "(Hζgmap & Hbs)".
+  1: apply map_disjoint_dom; eapply map_disjoint_dom in Hdisj; set_solver.
+  assert (ζ !! γ = None) as Hζγ.
+  1: eapply map_disjoint_Some_r; first done; apply lookup_insert.
+  iMod (lstore_own_insert with "Hζgmap") as "(Hζgmap & Hfrag)".
+  1: apply lookup_union_None; split; done.
+  rewrite insert_union_r; last done.
+  iModIntro.
+  iFrame "Hζgmap".
+  iApply big_sepM_insert; first done. iFrame.
 Qed.
 
 Lemma lstore_own_update γGS ζ γ b b' :
